No more axioms ...

compiler/proof_vec/equiv_poly1305_avx.ec
@@ -1,33 +1,146 @@
 require import AllCore IntDiv List CoreMap Jasmin_model.
 require import Poly1305_amd64_5x Poly1305_amd64_5xPR Poly1305_avx_5x Poly1305_avx_5xp.
+import StdOrder.IntOrder.
 
-axiom W128_unpack_2u64_of_uint i : 
-  unpack_2u64 (W128.of_uint i) = 
-    let i = i %% (2^ W128.size) in
-    (W64.of_uint (i %% 2^64), W64.of_uint (i %/ 2^64)).
+lemma zero_u128_pack : 
+  Poly1305_avx_5xp.zero_u128 = pack2 [W64.of_int 0; W64.of_int 0].
+proof. by rewrite of_uint_pack2. qed.
 
-hint simplify W128_unpack_2u64_of_uint.
+lemma five_u128_pack : 
+   Poly1305_avx_5xp.five_u128 = pack2 [W64.of_int 5; W64.of_int 5].
+proof. by rewrite of_uint_pack2. qed.
 
-axiom W64_unpack_2u32_of_uint i : 
-  unpack_2u32 (W64.of_uint i) = 
-    let i = i %% (2^ W64.size) in
-    (W32.of_uint (i %% 2^32), W32.of_uint (i %/ 2^32)).
-  
-hint simplify W64_unpack_2u32_of_uint.
+lemma bit25_u128_pack :
+   Poly1305_avx_5xp.bit25_u128 = pack2 [W64.of_int 16777216; W64.of_int 16777216].
+proof. by rewrite of_uint_pack2. qed.
 
-hint simplify (pack_unpack_2u64, unpack_pack_2u64)@0.
+lemma mask26_u128_pack1 :
+   Poly1305_avx_5xp.mask26_u128 = pack2 [W64.of_int 67108863; W64.of_int 67108863].
+proof. by rewrite of_uint_pack2. qed.
 
-hint simplify (iota0, iotaS_minus)@0.
+hint simplify (zero_u128_pack, five_u128_pack, bit25_u128_pack, mask26_u128_pack1).
 
-axiom nosmt W64_addw0 (w:W64.t) : w + W64.of_uint 0 = w. 
-axiom nosmt W64_addwA (x y z:W64.t) : x + (y + z) = x + y + z.
-axiom nosmt W64_addi x y : W64.of_uint x + W64.of_uint y = W64.of_uint (x + y).
-axiom nosmt W64_subi x y : W64.of_uint x - W64.of_uint y = W64.of_uint (x - y).
-axiom nosmt W64_shr_add i j (w:W64.t) : 0 <= i => 0 <= j => (* i + j <= 64 => *) w `>>>` i `>>>`j = w `>>>` (i+j).
+lemma and_small n : 0 <= n < 4294967296 => W64.of_int n `&` W64.of_int 4294967295 = W64.of_int n.
+proof. 
+  have -> h: 4294967295 = 2^32 - 1 by done. 
+  rewrite W64.and_mod //.
+  by rewrite W64.of_uintK modz_dvd 1:// modz_small 2://;apply bound_abs.
+qed.
 
-axiom W64_shr_or i (w1 w2 :W64.t) : (w1 `|` w2) `>>>` i = (w1 `>>>`i) `|` (w2 `>>>`i).
-axiom W64_shr_64 i (w:W64.t) : 64 <= i => w `>>>` i = W64.zeros.
-axiom W64_or0w w : W64.zeros `|` w = w.
+hint simplify and_small.
+
+lemma zeroext_truncateu64 (w:W64.t) :
+   zeroextu64 (truncateu32 w) = w `&` W64.of_int 4294967295.
+proof. by rewrite zeroext_truncateu32_and. qed.
+
+hint simplify zeroext_truncateu64. 
+
+(* ------------------------------------------------------------------------ *)
+
+op bounded n (w:W64.t) = W64.to_uint w < 2^n
+axiomatized by boundedE.
+
+lemma bounded_add i x y : 0 < i => bounded (i-1) x => bounded (i-1) y => bounded i (x + y).
+proof.
+  move=> hi; rewrite !boundedE (powS_minus 2 i) 1://.
+  rewrite W64.to_uintD; smt (W64.to_uint_cmp le_modz).
+qed.
+
+lemma bounded0 i : bounded i (W64.of_int 0).
+proof. by rewrite boundedE /= gt0_pow2. qed.
+
+lemma boundedNeg i w : i <= 0 => bounded i w <=> w = W64.of_int 0.
+proof.
+  move=> hi;rewrite boundedE powNeg 1:/#;split=> [|-> //].
+  rewrite -{2}(W64.to_uintK w)=> h.
+  by have -> : to_uint w = 0 by smt (W64.to_uint_cmp).
+qed.
+
+lemma bounded_mul i j x y:
+  bounded i x => 
+  bounded j y =>
+  bounded (i+j) (x * y).
+proof.
+  case: (0 < i) => hi;last first.
+  + by rewrite boundedNeg 1:/# => -> /= ?; apply bounded0.
+  case: (0 < j)=> hj;last first.
+  + by move=> ?; rewrite boundedNeg 1:/# => -> /=; apply bounded0.
+  rewrite !boundedE to_uintM -pow_add 1,2:ltzW 1,2:// => h1 h2. 
+  apply (ler_lt_trans (to_uint x * to_uint y)).
+  + by apply le_modz; smt (W64.to_uint_cmp). 
+  apply ltr_pmul => //; smt (W64.to_uint_cmp). 
+qed.
+
+lemma bounded_shr i j x : 
+  0 <= j < 64 => 0 <= i => 
+  bounded (i + j) x => 
+  bounded i (x `>>` W8.of_int j).
+proof.
+  rewrite !boundedE /W64.(`>>`) => -[h0j hjs] hi hx.
+  rewrite W8.of_uintK -pow2_6 modz_mod_pow2 /min /=.
+  rewrite modz_small 1:// W64.to_uint_shr 1://.
+  apply ltz_divLR; 1: by apply gt0_pow2.
+  by rewrite pow_add.
+qed.
+
+lemma boundedP n w :  
+  bounded n w <=> forall i, n <= i < W64.size => !w.[i].
+proof.
+  case (0 <= n) => hn.
+  + have -> : bounded n w <=> (to_uint w = (to_uint w) %% 2^n).
+    + rewrite boundedE;split => [h | ->].
+      + rewrite modz_small; smt (W64.to_uint_cmp).
+      smt (modz_cmp gt0_pow2).
+    have -> : to_uint w = to_uint w %% 2 ^ n <=> w = W64.of_int (to_uint w %% 2 ^ n).
+    + split => [<- | ->]; 1: by rewrite W64.to_uintK.
+      by rewrite of_uintK !modz_mod_pow2 /#. 
+    rewrite -W64.and_mod 1://.
+    split => [-> i hi| hi].
+    + by rewrite /= of_int_powm1 /#.
+    apply W64.wordP => i h0i /=;rewrite of_int_powm1 h0i.
+    by case (i < n) => hin //=; rewrite hi /#. 
+  rewrite boundedNeg 1:/#.
+  by split => [-> //| hi];apply W64.wordP => k hk /=;rewrite hi 2:// /#.
+qed.
+
+lemma bounded_and i x y : bounded i x \/ bounded i y => bounded i (x `&` y).
+proof. by rewrite !boundedP /= => -[] h j hj;rewrite h. qed.
+ 
+lemma bounded_or  i x y : bounded i x /\ bounded i y => bounded i (x `|` y).
+proof. by rewrite !boundedP /= => -[h1 h2] j hj;rewrite h1 // h2. qed.
+
+lemma bounded_weak (i j:int) x : i <= j => bounded i x => bounded j x.
+proof.
+  case : (0 <= i) => hi hij.
+  + by rewrite !boundedE; smt (pow_Mle).
+  by rewrite boundedNeg 1:/# => ->;apply bounded0.  
+qed.
+
+lemma bounded_w64 i w : 64 <= i => bounded i w.
+proof. by rewrite boundedE;smt (W64.to_uint_cmp pow_Mle). qed.
+
+lemma bounded_and_2p26 i w : 26 <= i => bounded i (w `&`  (W64.of_int 67108863)).
+proof.
+  move=> h; apply (bounded_weak 26); 1: done.
+  by apply bounded_and;right;rewrite boundedE. 
+qed.
+
+lemma bounded_and_2p32 i w : 32 <= i => bounded i (w `&` (W64.of_int 4294967295)).
+  move=> h; apply (bounded_weak 32); 1: done.
+  by apply bounded_and;right;rewrite boundedE. 
+qed.
+
+lemma bounded_mul5 i w : bounded (i-3) w => bounded i (w * (W64.of_int 5)).
+proof.
+  move=> h; have -> : i = (i - 3) + 3 by ring.
+  by apply bounded_mul => //; rewrite boundedE.
+qed.
+
+lemma bounded32_and w : bounded 32 w => w `&` (of_int 4294967295)%W64 = w.
+proof.
+  rewrite boundedE /= => h.
+  rewrite -(W64.to_uintK w) and_small 2://; smt (W64.to_uint_cmp).
+qed.
 
 (* ------------------------------------------------------------------------------ *)
 (* AVX-5x and its optimized version AVX-5xp                                       *)
@@ -55,9 +168,6 @@ equiv amd64_amd64_pr_load : Poly1305_amd64_5x.M.load ~ Poly1305_amd64_5xPR.M.loa
    ={Glob.mem, in_0} ==> ={res}.
 proof. sim. qed.
 
-axiom W64_subaddA (x y z:W64.t) : x - (y + z) = (x - y) + z.
-axiom W64_addsubA (x y z:W64.t) : x + (y - z) = (x + y) - z.
-
 equiv poly1305_amd64_amd64_pr : 
   Poly1305_amd64_5x.M.poly1305 ~ Poly1305_amd64_5xPR.M.poly1305 :
     ={arg,Glob.mem} ==> ={res, Glob.mem}.
@@ -78,17 +188,16 @@ proof.
     seq 7 10 : (#pre); 1:by sim.
     transitivity{1} {
         x0 <@ Poly1305_amd64_5x.M.load(in_0);
-        x1 <@ Poly1305_amd64_5x.M.load(in_0 + (of_uint 32)%W64);
-        y0 <@ Poly1305_amd64_5x.M.load((in_0 + (of_uint 16)%W64));
-        y1 <@ Poly1305_amd64_5x.M.load((in_0 +  (of_uint 32)%W64 + (of_uint 16)%W64));
-        in_0 <- (in_0 + (of_uint 32)%W64) + (of_uint 32)%W64;
+        x1 <@ Poly1305_amd64_5x.M.load(in_0 + (of_int 32)%W64);
+        y0 <@ Poly1305_amd64_5x.M.load((in_0 + (of_int 16)%W64));
+        y1 <@ Poly1305_amd64_5x.M.load((in_0 +  (of_int 32)%W64 + (of_int 16)%W64));
+        in_0 <- (in_0 + (of_int 32)%W64) + (of_int 32)%W64;
       } 
       (={Glob.mem, in_0, s_r2, s_r2x5} ==> ={in_0, x0, x1, y0, y1})
       (={Glob.mem, in_0, s_r2, s_r2x5} ==> ={in_0, x0, x1, y0, y1})=> //.
     + by move=> &m1 &m2 />; exists Glob.mem{m2} in_0{m2} s_r2{m2} s_r2x5{m2}.
     + do !(wp;call (_: ={Glob.mem, in_0} ==> ={res}); 1: by sim); skip => />.
-      move=> &m1. 
-      by rewrite -!W64_addsubA W64_subi -!W64_addwA !W64_addi.
+      move=> &m1; split => [|_]; 1: (by ring); split => [|_]; ring. 
     swap{1} 3 -1; do !(wp; call amd64_amd64_pr_load); auto => />.
 
   (* remaining_blocks *)
@@ -108,17 +217,17 @@ proof.
     seq 6 8 : (#pre); 1: by sim.
     transitivity{1} {
         x0 <@ Poly1305_amd64_5x.M.load(in_0);
-        x1 <@ Poly1305_amd64_5x.M.load(in_0 + (of_uint 32)%W64);
-        y0 <@ Poly1305_amd64_5x.M.load((in_0 + (of_uint 16)%W64));
-        y1 <@ Poly1305_amd64_5x.M.load((in_0 +  (of_uint 32)%W64 + (of_uint 16)%W64));
-        in_0 <- (in_0 + (of_uint 32)%W64) + (of_uint 32)%W64;
+        x1 <@ Poly1305_amd64_5x.M.load(in_0 + (of_int 32)%W64);
+        y0 <@ Poly1305_amd64_5x.M.load((in_0 + (of_int 16)%W64));
+        y1 <@ Poly1305_amd64_5x.M.load((in_0 +  (of_int 32)%W64 + (of_int 16)%W64));
+        in_0 <- (in_0 + (of_int 32)%W64) + (of_int 32)%W64;
       } 
       ( ={Glob.mem, hx, hy, in_0, s_r4, s_r4x5, s_r2, s_r2x5} ==> ={in_0, hy, y1, y0, x1, x0} )   
       ( ={Glob.mem, hx, hy, in_0, s_r4, s_r4x5, s_r2, s_r2x5} ==> ={in_0, hy, y1, y0, x1, x0} ) => //.
     + by move=> &m1 &m2 />; exists Glob.mem{m2} hx{m2} hy{m2} in_0{m2} s_r2{m2} s_r2x5{m2} s_r4{m2} s_r4x5{m2}.
     move=> />.
     + do !(wp;call (_: ={Glob.mem, in_0} ==> ={res}); 1: by sim); wp; skip => />.
-      by rewrite -!W64_addsubA W64_subi -!W64_addwA !W64_addi.
+      move=> &m1; split => [|_]; 1: (by ring); split => [|_]; ring. 
     by swap{1} 3 -1; do !(wp; call amd64_amd64_pr_load); auto => />.
 
   (* final_mul *)
@@ -134,28 +243,24 @@ qed.
 
 op rela4 (x y: W64.t Array4.t) 
      (xy : W128.t Array4.t) = 
-  xy.[0] = pack_2u64 (x.[0], y.[0]) /\
-  xy.[1] = pack_2u64 (x.[1], y.[1]) /\
-  xy.[2] = pack_2u64 (x.[2], y.[2]) /\
-  xy.[3] = pack_2u64 (x.[3], y.[3]).
+  xy.[0] = pack2 [x.[0]; y.[0]] /\
+  xy.[1] = pack2 [x.[1]; y.[1]] /\
+  xy.[2] = pack2 [x.[2]; y.[2]] /\
+  xy.[3] = pack2 [x.[3]; y.[3]].
 
 op rela5 (x y: W64.t Array5.t) 
      (xy : W128.t Array5.t) = 
-  xy.[0] = pack_2u64 (x.[0], y.[0]) /\
-  xy.[1] = pack_2u64 (x.[1], y.[1]) /\
-  xy.[2] = pack_2u64 (x.[2], y.[2]) /\
-  xy.[3] = pack_2u64 (x.[3], y.[3]) /\
-  xy.[4] = pack_2u64 (x.[4], y.[4]).
+  xy.[0] = pack2 [x.[0]; y.[0]] /\
+  xy.[1] = pack2 [x.[1]; y.[1]] /\
+  xy.[2] = pack2 [x.[2]; y.[2]] /\
+  xy.[3] = pack2 [x.[3]; y.[3]] /\
+  xy.[4] = pack2 [x.[4]; y.[4]].
 
 op is_x5 (z : W64.t Array5.t) (zx5 : W64.t Array4.t) = 
-  zx5.[0] = z.[1] * W64.of_uint 5 /\
-  zx5.[1] = z.[2] * W64.of_uint 5 /\
-  zx5.[2] = z.[3] * W64.of_uint 5 /\
-  zx5.[3] = z.[4] * W64.of_uint 5.
-
-op bounded n (w:W64.t) = 
-  W64.to_uint w < 2^n
-  axiomatized by boundedE.
+  zx5.[0] = z.[1] * W64.of_int 5 /\
+  zx5.[1] = z.[2] * W64.of_int 5 /\
+  zx5.[2] = z.[3] * W64.of_int 5 /\
+  zx5.[3] = z.[4] * W64.of_int 5.
 
 op wf5 (z : W64.t Array5.t) = 
    bounded 27 z.[0] /\
@@ -170,39 +275,6 @@ op wf4 (z : W64.t Array4.t) =
    bounded 30 z.[2] /\
    bounded 30 z.[3].
 
-axiom bounded_add i x y : 0 < i => bounded (i-1) x => bounded (i-1) y => bounded i (x + y).
-axiom bounded_and i x y : bounded i x \/ bounded i y => bounded i (x `&` y).
-axiom bounded_or  i x y : bounded i x /\ bounded i y => bounded i (x `|` y).
-
-axiom bounded_shr i j x : 
-  0 <= i => (* i + j <= 64 => *)
-  bounded (i + j) x => 
-  bounded i (x `>>` W8.of_uint j).
-axiom bounded_mul i j x y:
-  bounded i x => 
-  bounded j y =>
-  bounded (i+j) (x * y).
-
-axiom bounded_weak (i j:int) x : i <= j => bounded i x => bounded j x.
-
-axiom bounded_w64 i w : 64 <= i => bounded i w.
-
-lemma bounded_and_2p26 i w : 26 <= i => bounded i (w `&`  (W64.of_uint 67108863)).
-proof.
-  move=> h; apply (bounded_weak 26); 1: done.
-  by apply bounded_and;right;rewrite boundedE. 
-qed.
-
-lemma bounded_and_2p32 i w : 32 <= i => bounded i (w `&` (W64.of_uint 4294967295)).
-  move=> h; apply (bounded_weak 32); 1: done.
-  by apply bounded_and;right;rewrite boundedE. 
-qed.
-
-lemma bounded_mul5 i w : bounded (i-3) w => bounded i (w * (W64.of_uint 5)).
-proof.
-  move=> h; have -> : i = (i - 3) + 3 by ring.
-  by apply bounded_mul => //; rewrite boundedE.
-qed.
 
 hoare carry_reduceWF : Poly1305_amd64_5xPR.M.carry_reduce : true ==> wf5 res.
 proof.
@@ -217,31 +289,6 @@ proof.
   by proc; wp; skip => &m1 &m2 /= ->.
 qed.
 
-axiom pack_mulu_32 w1 w2 : 
-  pack_2u32 (W32.mulu w1 w2) = (zeroext_32_64 w1) * (zeroext_32_64 w2).
-
-hint simplify pack_mulu_32.
-
-axiom zeroext_and2p32 w : zeroext_32_64 (unpack_2u32 w).`1 = w `&` W64.of_uint 4294967295.
-
-lemma zeroext_of_uint i : zeroext_32_64 (W32.of_uint i) = W64.of_uint (i %% W32.modulus).
-proof. by rewrite zeroext_32_64E. qed.
-
-hint simplify zeroext_of_uint.
-
-hint simplify (VPAND_128_64, VPOR_128_64, VPXOR_128_64)@0. 
-
-lemma VPAND_128_64_l w1 w2 : 
-   pack_2u64 w1 `&` w2 = 
-     pack_2u64(w1.`1 `&` (unpack_2u64 w2).`1, w1.`2 `&` (unpack_2u64 w2).`2).
-proof. by rewrite -(pack_unpack_2u64 w2) VPAND_128_64. qed.
-
-lemma VPOR_128_64_l w1 w2 : 
-   pack_2u64 w1 `|` w2 = 
-     pack_2u64(w1.`1 `|` (unpack_2u64 w2).`1, w1.`2 `|` (unpack_2u64 w2).`2).
-proof. by rewrite -(pack_unpack_2u64 w2) VPOR_128_64. qed.
-
-hint simplify (VPAND_128_64_l, VPOR_128_64_l)@1.
 
 equiv carry_reduce_u128P : Poly1305_amd64_5xPR.M.carry_reduce_u128 ~ Poly1305_avx_5x.M.carry_reduce_u128 : 
         rela5 hx{1} hy{1} x{2} ==>
@@ -250,8 +297,7 @@ proof.
   conseq (_: rela5 res{1}.`1 res{1}.`2 res{2}) (_ : true ==> wf5 res.`1 /\ wf5 res.`2) => //.
   + by proc; do 2!call carry_reduceWF;auto.
   proc. inline *. wp; skip;rewrite /rela5 => /=. 
-  move=> &m1 &m2 [#] 5!->. cbv delta.  
-  by rewrite -!zeroext_and2p32.
+  by move=> &m1 &m2 [#] 5!-> /=; cbv x86_VPADD_2u64 x86_VPMULU_128 (%/) (%%) mulu_64.
 qed.
 
 hoare clampWF : Poly1305_amd64_5xPR.M.clamp : true ==> wf5 res.
@@ -288,8 +334,6 @@ proof.
   + by move=> ?????;rewrite !Array5.ext_eq_all.
   by unroll for {2} 5; wp; skip => &m1 &m2; cbv delta => [#] 5!->.
 qed.
-
-axiom zeroext_bounded w : bounded 32 w => zeroext_32_64 (unpack_2u32 w).`1 = w.
  
 equiv mulmod_u128P : 
   Poly1305_amd64_5xPR.M.mulmod_u128 ~ Poly1305_avx_5x.M.mulmod_u128 : 
@@ -299,11 +343,12 @@ equiv mulmod_u128P :
   rela4 y1x5{1} y2x5{1} yx5{2} ==>
   rela5 res{1}.`1 res{1}.`2 res{2}.
 proof.
-  proc => /=; inline *; wp; skip; cbv delta.
+  proc => /=; inline *; wp; skip.
+ cbv x86_VPMULU_128 x86_VPADD_2u64 wf5 wf4 rela5 rela4 mulu_64.
   move=> &m1 &m2 [#] X10 X11 X12 X13 X14 X20 X21 X22 X23 X24.
   move=> Y10 Y11 Y12 Y13 Y14 Y20 Y21 Y22 Y23 Y24.
   move=> Y1x0 Y1x1 Y1x2 Y1x3 Y2x0 Y2x1 Y2x2 Y2x3 14!-> /=.
-  smt (zeroext_bounded bounded_weak).
+  smt (bounded32_and bounded_weak).
 qed.
 
 equiv mulmod_add_u128P : 
@@ -318,10 +363,10 @@ proof.
   proc => /=; inline *. 
   unroll for{1} 107. unroll for{1} 20.
   unroll for{2} 11.
-  wp; skip; cbv delta.
+  wp; skip; cbv x86_VPMULU_128 x86_VPADD_2u64 wf5 wf4 rela5 rela4 mulu_64.
   move=> &m1 &m2 [#] X10 X11 X12 X13 X14 X20 X21 X22 X23 X24.
   move=> Y0 Y1 Y2 Y3 Y4 Yx0 Yx1 Yx2 Yx3 19!-> /=.
-  smt (zeroext_bounded bounded_weak).
+  smt (bounded32_and bounded_weak).
 qed.
 
 equiv add_u128P : Poly1305_amd64_5xPR.M.add_u128 ~ Poly1305_avx_5x.M.add_u128 :  
@@ -338,10 +383,11 @@ qed.
 hoare loadWF : Poly1305_amd64_5xPR.M.load : true ==> wf5 res.
 proof.
   proc; inline *; wp; skip; rewrite /wf5 => /= &hr.
-  have h : bounded 27 ((of_uint 16777216))%W64 by rewrite boundedE. 
+  have h : bounded 27 ((of_int 16777216))%W64 by rewrite boundedE. 
   smt (bounded_and_2p26 bounded_add bounded_shr bounded_w64 bounded_or).
 qed.
 
+hint simplify (W64.get_out, W64.of_intwE). 
 equiv unpack_u128P : 
  Poly1305_amd64_5xPR.M.unpack_u128x2_to_u26x5x2 ~  Poly1305_avx_5x.M.unpack_u128x2_to_u26x5x2 :
   ={Glob.mem} /\ in_0{1} = m{2} ==> rela5 res{1}.`1 res{1}.`2 res{2} /\ wf5 res{1}.`1 /\ wf5 res{1}.`2.
@@ -349,10 +395,10 @@ proof.
   conseq (_: ={Glob.mem} /\ in_0{1} = m{2} ==> rela5 res{1}.`1 res{1}.`2 res{2}) 
          (_: true ==> wf5 res.`1 /\ wf5 res.`2).
   + by proc; do !(call loadWF;wp); skip.
-  proc;inline *;wp; skip => />; cbv delta => &1.
-  rewrite !W64_addw0 -!W64_addwA W64_addi /= !W64_shr_add //=.
-  rewrite !W64_shr_or !W64_shr_add //= !(W64_shr_64 78) //= !W64_or0w.
-  admit. (* it is true since we look only on the low bit *)
+  proc;inline *;wp; skip => />.
+  cbv x86_VPUNPCKL_2u64 x86_MOVD_64 (%/) (%%).
+  move => &m.
+  by split; apply W128.all_eq_eq;cbv W128.all_eq (%%) (%/) W64.(`>>`) W64.(`<<`) W64.int_bit. 
 qed.
 
 equiv remaining_blocksP : Poly1305_amd64_5xPR.M.remaining_blocks ~ Poly1305_avx_5x.M.remaining_blocks :
@@ -409,14 +455,7 @@ phoare unpack_u26x5x2P x0 y0:
     s = x0 /\ t = y0 ==> rela5 x0 y0 res] = 1%r.
 proof.
   proc.
-  (* FIXME "unroll for 3", should work *)
-  unroll 3; rcondt 3; 1: by auto.
-  unroll 7; rcondt 7; 1: by auto.
-  unroll 11; rcondt 11; 1: by auto.
-  unroll 15; rcondt 15; 1: by auto.
-  unroll 19; rcondt 19; 1: by auto.
-  rcondf 23; 1: by auto.
-  wp;skip;cbv delta => />.
+  by unroll for 3; wp;skip => />; cbv x86_VPINSR_2u64.
 qed.
 
 equiv poly1305_amd64_avx_5x :
@@ -438,15 +477,15 @@ proof.
   + by skip => &m1 &m2 /> R0 R1 R2 R3 R4 4!->; rewrite !bounded_mul5.
   seq 4 4 : (#pre /\ ={b64}); 1: by sim />.
   if => //.
-  seq 0 0 : (#[/:-1]pre); 1: by auto. 
-  seq 5 5 : (#pre /\ ={r2, s_b64, s_r2} /\ (r2 = s_r2){1} /\ wf5 r2{1}).
+  seq 1 1 : (#pre /\ ={s_b64} /\ (b64 = s_b64){1}); 1: by auto.
+  seq 4 4 : (#pre /\  ={r2, s_r2} /\ (r2 = s_r2){1} /\ wf5 r2{1}).
   + conseq |>; wp; call carry_reduceP.
-    by conseq (_: ={r2, s_b64}) => //; sim.
+    by conseq (_: ={r2}) => //; sim.
   seq 2 2 : (#pre /\ (is_x5 r2 s_r2x5){1}).
   + conseq />;unroll for {1} 2; unroll for {2} 2.
     by wp;skip;cbv delta => />.
   seq 0 0 : (#pre /\ wf4 s_r2x5{1}).
-  + by skip => &m1 &m2 |> ? ? ? />  R0 R1 R2 R3 R4 4!->; rewrite !bounded_mul5.
+  + by skip => &m1 &m2 |> ? ? ? ? />  R0 R1 R2 R3 R4 4!->; rewrite !bounded_mul5.
   seq 0 1 : (#pre); 1: by auto.
   seq 0 2 : (#pre /\ (r2r = s_r2r){2} /\ rela5 r2{1} r{1} r2r{2}).
   + wp.
@@ -454,19 +493,19 @@ proof.
     by call{2} (unpack_u26x5x2P r2_R r_R); skip => />.
   seq 0 2 : (#pre /\ rela4 s_r2x5{1} s_rx5{1} s_r2rx5{2}).
   + conseq />;unroll for {2} 2.
-    wp;skip => |> &m2 + + _ + + _.
-    move=> /> R0 R1 R2 R3 R4 4!-> R20 R21 R22 R23 R24 4!->  ? 4!->.
-    cbv delta; smt (zeroext_bounded bounded_weak).
+    wp;skip => |> &m2 + + _ _ + + _.
+    move=> />  R0 R1 R2 R3 R4 4!-> R20 R21 R22 R23 R24 4!-> ? 4!->.
+    by cbv x86_VPMULU_128 (%%) (%/) mulu_64; smt (bounded32_and bounded_weak).
   seq 0 2 : (#pre /\ (r2r2 = s_r2r2){2} /\ rela5 r2{1} r2{1} r2r2{2}).
   + wp; conseq />.
     exists * r2{2}; elim * => r2_R.
     by call{2} (unpack_u26x5x2P r2_R r2_R); skip => />.
   seq 0 2 : (#pre /\ rela4 s_r2x5{1} s_r2x5{1} s_r2r2x5{2}).
   + conseq />;unroll for {2} 2.
-    wp;skip => |> &m _ _ _ + + _ _ _.
+    wp;skip => |> &m _ _ _ _ + + _ _ _.
     move=> /> ?????  4!-> ? 4!->.  
-    cbv delta; smt (zeroext_bounded bounded_weak).
-  seq 1 1 : (#pre /\ (b64 = s_b64){1}); 1: by auto. 
+    cbv x86_VPMULU_128 (%%) (%/) mulu_64; smt (bounded32_and bounded_weak).
+  seq 1 1 : (#pre); 1: by auto. 
   if => //.
   + seq 4 3 : (#pre /\ ={r4} /\ (r4 = s_r4){1} /\ wf5 r4{1}).
     + conseq |>; wp;call carry_reduceP.
@@ -476,10 +515,10 @@ proof.
       by call{2} (unpack_u26x5x2P r4_R r4_R); skip => />.
     seq 2 2 : (#pre /\ is_x5 r4{1} s_r4x5{1} /\ rela4 s_r4x5{1} s_r4x5{1} s_r4r4x5{2}).
     + unroll for {1} 2. unroll for {2} 2.
-      wp; skip => |> &m1 &m2 _ _ _ _ _ _ _ _ _ _ _ /> ????? ? 4!->. 
-      cbv delta; smt (zeroext_bounded bounded_weak).
+      wp; skip => |> &m1 &m2 _ _ _ _ _ _ _ _ _ _ _ _ /> ????? ? 4!->. 
+      cbv x86_VPMULU_128 (%%) (%/) mulu_64; smt (bounded32_and bounded_weak).
     seq 0 0 : (#pre /\ wf4 s_r4x5{1}).
-    + skip => &m1 &m2 |> ??????????? + _ + _.
+    + skip => &m1 &m2 |> ???????????? + _ + _.
       by move=> /> ????? 4!->; rewrite !bounded_mul5.
     call final_mulP => /=.
     while (={Glob.mem, b64, in_0} /\ 
@@ -495,11 +534,14 @@ proof.
     by wp; call first_blockP; wp; skip.  
   rcondf{1} 5.  
   + move=> &m2; wp; conseq (_: true) => //.
-    move=> |> ??????????. 
-    admit. (* fact on comparison *)
+    move=> |> ??? + ???????. 
+    rewrite -!uleNgt !W64.uleE W64.ultE /= => h.
+    rewrite to_uint_minus 1:W64.uleE /= /#. 
   rcondf{2} 5.
   + move=> &m1; wp; conseq (_: true) => //.
-    move=> |> ???????????.  admit. 
+    move=> |> ???? + ???????.  
+    rewrite -!uleNgt !W64.uleE W64.ultE /= => h.
+    rewrite to_uint_minus 1:W64.uleE /= /#. 
   by call final_mulP; wp; call first_blockP; wp; skip.  
 qed.
 
