compiler/proof_vec/poly1305_avx_5xp_ct_proof.ec
@@ -4,5 +4,6 @@ require import Jasmin_model Poly1305_avx_5xp_ct.
 proc; inline *;sim.
 *)
 
-equiv poly1305_ct : M.poly1305 ~ M.poly1305 : ={k, inlen, in_0, out, M.leakages} ==> ={M.leakages}.
+equiv poly1305_ct : M.poly1305 ~ M.poly1305 : 
+  ={k, inlen, in_0, out, M.leakages} ==> ={M.leakages}.
 proof. proc => /=; inline *; sim. qed.
